LL1/Proofs/ParseTableGen/mkParseTableEntries_Correctness.v
@@ -1,0 +1,53 @@
+Require Import List.
+
+Require Import Lib.Grammar.
+
+Require Import LL1.ParseTable.
+Require Import LL1.ParseTableGen.
+
+Definition pt_entries_correct ps g :=
+  forall x la gamma,
+    In (x, la, gamma) ps <-> lookahead_for la x gamma g.
+
+Definition entries_correct_wrt_production g es x gamma :=
+  forall la, In (x, la, gamma) es <-> lookahead_for la x gamma g.
+
+(* invariant relating a list of entries to a list of productions *)
+Inductive entries_correct_wrt_productions (g : grammar) :
+  list pt_entry -> list production -> Prop :=
+| EntriesCorrect_nil : 
+    entries_correct_wrt_productions g nil nil
+| EntriesCorrect_cons :
+    forall front_entries back_entries x gamma ps,
+      entries_correct_wrt_productions g back_entries ps
+      -> entries_correct_wrt_production g front_entries x gamma
+      -> entries_correct_wrt_productions g (front_entries ++ back_entries) ((x, gamma) :: ps).
+    
+Lemma invariant_iff_pt_entries_correct :
+  forall es g,
+    entries_correct_wrt_productions g es (productions g) <-> pt_entries_correct es g.
+Proof.
+Admitted.
+
+Lemma mkParseTableEntries'_sound :
+  forall g nu fi fo ps es,
+    mkParseTableEntries' nu fi fo ps = es
+    -> entries_correct_wrt_productions g es ps.
+Proof.
+Admitted.
+  
+Lemma mkParseTableEntries_sound :
+  forall g nu fi fo es,
+    nullable_set_for nu g
+    -> first_map_for fi g
+    -> follow_map_for fo g
+    -> mkParseTableEntries nu fi fo g = es
+    -> pt_entries_correct es g.
+Proof.
+  intros g nu fi fo es Hnu Hfi Hfo Hmk.
+  apply invariant_iff_pt_entries_correct.
+  unfold mkParseTableEntries in Hmk.
+  eapply mkParseTableEntries'_sound; eauto.
+Qed.
+    
+    
